revert to b751a5989

assembler/RelocProgSemantics.v
@@ -11,7 +11,7 @@ Require Import Asm RelocProg RelocProgram Globalenvs.
 Require Import Locations Stacklayout Conventions.
 Require Import Linking Errors.
 Require Import LocalLib.
-Require Import RelocProgGlobalenvs.
+Require Import RelocProgGlobalenvs RelocProgSemanticsArchi.
 
 Remark in_norepet_unique_r:
   forall T (gl: list (ident * T)) id g,
@@ -32,7 +32,42 @@ Section WITH_INSTR_SIZE.
   
 (** Small step semantics *)
 
-  
+(* I think it is almost the same in all architectures*)
+
+Inductive step (ge: Genv.t) : state -> trace -> state -> Prop :=
+| exec_step_internal:
+    forall b ofs i rs m rs' m',
+      rs PC = Vptr b ofs ->
+      Genv.find_ext_funct ge (Vptr b ofs) = None ->
+      Genv.find_instr ge (Vptr b ofs) = Some i ->
+      exec_instr ge i rs m = Next rs' m' ->
+      step ge (State rs m) E0 (State rs' m')
+| exec_step_builtin:
+    forall b ofs ef args res rs m vargs t vres rs' m',
+      rs PC = Vptr b ofs ->
+      Genv.find_ext_funct ge (Vptr b ofs) = None ->
+      Genv.find_instr ge (Vptr b ofs) = Some (Pbuiltin ef args res)  ->
+      eval_builtin_args preg ge rs (rs RSP) m args vargs ->
+      external_call ef (Genv.genv_senv ge) vargs m t vres m' ->
+      rs' = nextinstr_nf (Ptrofs.repr (instr_size (Pbuiltin ef args res)))
+                         (set_res res vres
+                                  (undef_regs (map preg_of (destroyed_by_builtin ef)) rs)) ->
+        step ge (State rs m) t (State rs' m')
+| exec_step_external:
+    forall b ofs ef args res rs m t rs' m',
+      rs PC = Vptr b ofs ->
+      Genv.find_ext_funct ge (Vptr b ofs) = Some ef ->
+      forall ra (LOADRA: Mem.loadv Mptr m (rs RSP) = Some ra)
+        (RA_NOT_VUNDEF: ra <> Vundef)
+        (ARGS: extcall_arguments (rs # RSP <- (Val.offset_ptr (rs RSP) (Ptrofs.repr (size_chunk Mptr)))) m (ef_sig ef) args),
+        external_call ef (Genv.genv_senv ge) args m t res m' ->
+          rs' = (set_pair (loc_external_result (ef_sig ef)) res
+                          (undef_caller_save_regs rs))
+                  #PC <- ra
+                  #RA <- Vundef
+                  #RSP <- (Val.offset_ptr (rs RSP) (Ptrofs.repr (size_chunk Mptr))) ->
+        step ge (State rs m) t (State rs' m').
+
 (** Initialization of the global environment *)
 Definition gen_global (id:ident) (e:symbentry) : (block*ptrofs) :=
   match e.(symbentry_secindex) with
@@ -383,18 +418,21 @@ Fixpoint load_store_init_data (m: mem) (b: block) (p: Z) (il: list init_data) {s
 
 (* unchanged properties *)
 
+
 Remark store_init_data_unchanged:
   forall (P: block -> Z -> Prop) b i m p m',
   store_init_data m b p i = Some m' ->
   (forall ofs, p <= ofs < p + init_data_size i -> ~ P b ofs) ->
   Mem.unchanged_on P m m'.
 Proof.
-  intros. destruct i;simpl in *.
-  1-7 :try (eapply Mem.store_unchanged_on; eauto; fail).  
+  intros. destruct i; simpl in *;
+            try (eapply Mem.store_unchanged_on; eauto; fail).
   eapply Genv.store_zeros_unchanged;eauto.
-  (* Mptr: auto would simplify ptr.64 and I don't know how to solve it (Opaque dose not work) *)
-  eapply Mem.store_unchanged_on. eauto.
-  unfold Mptr. destruct Archi.ptr64;simpl;auto.
+  
+  (* destruct (Genv.find_symbol ge i); try congruence. *)
+  (* destruct p0. *)
+  (* eapply Mem.store_unchanged_on; eauto; *)
+  (* unfold Mptr; destruct Archi.ptr64; eauto. *)
 Qed.
 
 Remark store_init_data_list_unchanged:
@@ -592,19 +630,14 @@ Proof.
     split. rewrite <- H1; auto.
     rewrite  <- H2. auto.
     exists m'; auto. }
-  destruct i.
-  1-7: eauto.
-  (* store zero *)
+  destruct i; eauto.
   simpl. eapply Genv.store_zeros_exists.
   simpl in H. auto.
 
-  (* Mptr *)
-  simpl. eapply DFL.
-  unfold Mptr. simpl. destruct Archi.ptr64;auto.
-  unfold Mptr. simpl. destruct Archi.ptr64;auto.
   (* simpl. exploit H1; eauto. intros (b1 & OFS & FS). rewrite FS. eapply DFL. *)
   (* unfold init_data_size, Mptr. destruct Archi.ptr64; auto. *)
-  (* unfold Genv.init_data_alignment, Mptr. destruct Archi.ptr64; auto. *)                                                            
+  (* unfold Genv.init_data_alignment, Mptr. destruct Archi.ptr64; auto. *)
+                                                            
 Qed.
 
 (* SACC
@@ -2597,96 +2630,98 @@ Proof.
     inv H0. auto.
 Qed.
 
+  
+Inductive initial_state_gen {D: Type} (p: RelocProg.program fundef unit instruction D) (rs: regset) m: state -> Prop :=
+| initial_state_gen_intro:
+    forall m1 m2 stk
+      (MALLOC: Mem.alloc m 0 (max_stacksize + align (size_chunk Mptr) 8) = (m1,stk))
+      (MST: Mem.storev Mptr m1 (Vptr stk (Ptrofs.repr (max_stacksize + align (size_chunk Mptr) 8 - size_chunk Mptr))) Vnullptr = Some m2),
+      let ge := (globalenv p) in
+      let rs0 :=
+          rs # PC <- (Genv.symbol_address ge p.(prog_main) Ptrofs.zero)
+           # RA <- Vnullptr
+           # RSP <- (Vptr stk (Ptrofs.sub (Ptrofs.repr (max_stacksize + align (size_chunk Mptr) 8)) (Ptrofs.repr (size_chunk Mptr)))) in
+      initial_state_gen p rs m (State rs0 m2).
 
-(** New defined eval_builtin_arg for Genv.t *)
-Section EVAL_BUILTIN_ARG.
 
-Variable A: Type.
+Inductive initial_state (prog: program) (rs: regset) (s: state): Prop :=
+| initial_state_intro: forall m,
+    init_mem prog = Some m ->
+    initial_state_gen prog rs m s ->
+    initial_state prog rs s.
 
-Variable ge: Genv.t.
-Variable e: A -> val.
-Variable sp: val.
-Variable m:mem. 
+Inductive final_state: state -> int -> Prop :=
+  | final_state_intro: forall rs m r,
+      rs#PC = Vnullptr ->
+      rs#RAX = Vint r ->
+      final_state (State rs m) r.
 
-Inductive eval_builtin_arg: builtin_arg A -> val -> Prop :=
-  | eval_BA: forall x,
-      eval_builtin_arg (BA x) (e x)
-  | eval_BA_int: forall n,
-      eval_builtin_arg (BA_int n) (Vint n)
-  | eval_BA_long: forall n,
-      eval_builtin_arg (BA_long n) (Vlong n)
-  | eval_BA_float: forall n,
-      eval_builtin_arg (BA_float n) (Vfloat n)
-  | eval_BA_single: forall n,
-      eval_builtin_arg (BA_single n) (Vsingle n)
-  | eval_BA_loadstack: forall chunk ofs v,
-      Mem.loadv chunk m (Val.offset_ptr sp ofs) = Some v ->
-      eval_builtin_arg (BA_loadstack chunk ofs) v
-  | eval_BA_addrstack: forall ofs,
-      eval_builtin_arg (BA_addrstack ofs) (Val.offset_ptr sp ofs)
-  | eval_BA_loadglobal: forall chunk id ofs v,
-      Mem.loadv chunk m  (Genv.symbol_address ge id ofs) = Some v ->
-      eval_builtin_arg (BA_loadglobal chunk id ofs) v
-  | eval_BA_addrglobal: forall id ofs,
-      eval_builtin_arg (BA_addrglobal id ofs) (Genv.symbol_address ge id ofs)
-  | eval_BA_splitlong: forall hi lo vhi vlo,
-      eval_builtin_arg hi vhi -> eval_builtin_arg lo vlo ->
-      eval_builtin_arg (BA_splitlong hi lo) (Val.longofwords vhi vlo)
-  | eval_BA_addptr: forall a1 a2 v1 v2,
-      eval_builtin_arg a1 v1 ->
-      eval_builtin_arg a2 v2 ->
-      eval_builtin_arg (BA_addptr a1 a2) (if Archi.ptr64 then Val.addl v1 v2 else Val.add v1 v2).
+(* Local Existing Instance mem_accessors_default. *)
 
-                       
-Definition eval_builtin_args (al: list (builtin_arg A)) (vl: list val) : Prop :=
-  list_forall2 eval_builtin_arg al vl.
+Definition semantics (p: program) (rs: regset) :=
+  Semantics_gen step (initial_state p rs) final_state (globalenv p) (Genv.genv_senv (globalenv p)).
 
-Lemma eval_builtin_arg_determ:
-  forall a v, eval_builtin_arg a v -> forall v', eval_builtin_arg a v' -> v' = v.
+(** Determinacy of the [Asm] semantics. *)
+
+Lemma semantics_determinate: forall p rs, determinate (semantics p rs).
 Proof.
-  induction 1; intros v' EV; inv EV; try congruence.
-  f_equal; eauto.
-  destruct Archi.ptr64;f_equal;auto.
+Ltac Equalities :=
+  match goal with
+  | [ H1: ?a = ?b, H2: ?a = ?c |- _ ] =>
+      rewrite H1 in H2; inv H2; Equalities
+  | _ => idtac
+  end.
+  intros; constructor; simpl; intros.
+- (* determ *)
+  inv H; inv H0; Equalities.
++ split. constructor. auto.
++ discriminate.
++ discriminate.
++ assert (vargs0 = vargs) by (eapply eval_builtin_args_determ; eauto). subst vargs0.
+  exploit external_call_determ. eexact H5. eexact H11. intros [A B].
+  split. auto. intros. destruct B; auto. subst. auto.
++ assert (args0 = args) by (eapply Asm.extcall_arguments_determ; eauto). subst args0.
+  exploit external_call_determ. eexact H3. eexact H7. intros [A B].
+  split. auto. intros. destruct B; auto. subst. auto.
+- (* trace length *)
+  red; intros; inv H; simpl.
+  lia.
+  eapply external_call_trace_length; eauto.
+  eapply external_call_trace_length; eauto.
+- (* initial states *)
+  inv H; inv H0. assert (m = m0) by congruence. subst. inv H2; inv H3.
+  assert (m1 = m3 /\ stk = stk0) by intuition congruence. destruct H0; subst.
+  assert (m2 = m4) by congruence. subst.
+  f_equal. (* congruence. *)
+- (* final no step *)
+  assert (NOTNULL: forall b ofs, Vnullptr <> Vptr b ofs).
+  { intros; unfold Vnullptr; destruct Archi.ptr64; congruence. }
+  inv H. red; intros; red; intros. inv H; rewrite H0 in *; eelim NOTNULL; eauto.
+- (* final states *)
+  inv H; inv H0. congruence.
 Qed.
 
-Lemma eval_builtin_args_determ:
-  forall al vl, eval_builtin_args al vl -> forall vl', eval_builtin_args al vl' -> vl' = vl.
+Theorem reloc_prog_single_events p rs:
+  single_events (semantics p rs).
 Proof.
-  induction 1; intros v' EV; inv EV; f_equal; eauto using eval_builtin_arg_determ.
+  red. simpl. intros s t s' STEP.
+  inv STEP; simpl. lia.
+  eapply external_call_trace_length; eauto.
+  eapply external_call_trace_length; eauto.
 Qed.
 
- 
-End EVAL_BUILTIN_ARG.
-
-Hint Constructors eval_builtin_arg: barg.
-
-(* same lemmas as the in Events *)
-Section EVAL_BUILTIN_ARG_PRESERVED.
-
-Variables A: Type.
-Variable ge1: Genv.t.
-Variable ge2: Genv.t.
-Variable e: A -> val.
-Variable sp: val.
-Variable m: mem.
-
-Hypothesis symbols_preserved:
-  forall id, Genv.find_symbol ge2 id = Genv.find_symbol ge1 id.
-
-Lemma eval_builtin_arg_preserved:
-  forall a v, eval_builtin_arg A ge1 e sp m a v -> eval_builtin_arg A ge2 e sp m a v.
+Theorem reloc_prog_receptive p rs:
+  receptive (semantics p rs).
 Proof.
-   assert (EQ: forall id ofs, Genv.symbol_address ge2 id ofs = Genv.symbol_address ge1 id ofs).
-  { unfold Genv.symbol_address; simpl; intros. rewrite symbols_preserved; auto. }
-  induction 1; eauto with barg. rewrite <- EQ in H; eauto with barg. rewrite <- EQ; eauto with barg.
+  split.
+  - simpl. intros s t1 s1 t2 STEP MT.
+    inv STEP.
+    inv MT. eexists. eapply exec_step_internal; eauto.
+    edestruct external_call_receptive as (vres2 & m2 & EC2); eauto.
+    eexists. eapply exec_step_builtin; eauto.
+    edestruct external_call_receptive as (vres2 & m2 & EC2); eauto.
+    eexists. eapply exec_step_external; eauto.
+  - eapply reloc_prog_single_events; eauto.
 Qed.
-
-Lemma eval_builtin_args_preserved:
-  forall al vl, eval_builtin_args A ge1 e sp m al vl -> eval_builtin_args A ge2 e sp m al vl.
-Proof.
-  induction 1; constructor; auto; eapply eval_builtin_arg_preserved; eauto.
-Qed.
-
-End EVAL_BUILTIN_ARG_PRESERVED.
 
 End WITH_INSTR_SIZE.
