x86/RelocProgSemanticsArchi.v
@@ -4,7 +4,7 @@ Require Import Asm RelocProg RelocProgram Globalenvs.
 Require Import Locations Stacklayout Conventions.
 Require Import Linking Errors.
 Require Import LocalLib.
-Require Import RelocProgGlobalenvs RelocProgSemantics0.
+Require Import RelocProgGlobalenvs.
 
 (** Evaluating an addressing mode *)
 
@@ -563,130 +563,101 @@ Proof.
   destruct p. eapply symbol_address_pres;eauto.
 Qed.
 
-Inductive step (ge: Genv.t) : state -> trace -> state -> Prop :=
-| exec_step_internal:
-    forall b ofs i rs m rs' m',
-      rs PC = Vptr b ofs ->
-      Genv.find_ext_funct ge (Vptr b ofs) = None ->
-      Genv.find_instr ge (Vptr b ofs) = Some i ->
-      exec_instr ge i rs m = Next rs' m' ->
-      step ge (State rs m) E0 (State rs' m')
-| exec_step_builtin:
-    forall b ofs ef args res rs m vargs t vres rs' m',
-      rs PC = Vptr b ofs ->
-      Genv.find_ext_funct ge (Vptr b ofs) = None ->
-      Genv.find_instr ge (Vptr b ofs) = Some (Pbuiltin ef args res)  ->
-      eval_builtin_args preg ge rs (rs RSP) m args vargs ->
-      external_call ef (Genv.genv_senv ge) vargs m t vres m' ->
-      rs' = nextinstr_nf (Ptrofs.repr (instr_size (Pbuiltin ef args res)))
-                         (set_res res vres
-                                  (undef_regs (map preg_of (destroyed_by_builtin ef)) rs)) ->
-        step ge (State rs m) t (State rs' m')
-| exec_step_external:
-    forall b ofs ef args res rs m t rs' m',
-      rs PC = Vptr b ofs ->
-      Genv.find_ext_funct ge (Vptr b ofs) = Some ef ->
-      forall ra (LOADRA: Mem.loadv Mptr m (rs RSP) = Some ra)
-        (RA_NOT_VUNDEF: ra <> Vundef)
-        (ARGS: extcall_arguments (rs # RSP <- (Val.offset_ptr (rs RSP) (Ptrofs.repr (size_chunk Mptr)))) m (ef_sig ef) args),
-        external_call ef (Genv.genv_senv ge) args m t res m' ->
-          rs' = (set_pair (loc_external_result (ef_sig ef)) res
-                          (undef_caller_save_regs rs))
-                  #PC <- ra
-                  #RA <- Vundef
-                  #RSP <- (Val.offset_ptr (rs RSP) (Ptrofs.repr (size_chunk Mptr))) ->
-        step ge (State rs m) t (State rs' m').
-
-
-Inductive initial_state_gen {D: Type} (p: RelocProg.program fundef unit instruction D) (rs: regset) m: state -> Prop :=
-| initial_state_gen_intro:
-    forall m1 m2 stk
-      (MALLOC: Mem.alloc m 0 (max_stacksize + align (size_chunk Mptr) 8) = (m1,stk))
-      (MST: Mem.storev Mptr m1 (Vptr stk (Ptrofs.repr (max_stacksize + align (size_chunk Mptr) 8 - size_chunk Mptr))) Vnullptr = Some m2),
-      let ge := (globalenv p) in
-      let rs0 :=
-          rs # PC <- (Genv.symbol_address ge p.(prog_main) Ptrofs.zero)
-           # RA <- Vnullptr
-           # RSP <- (Vptr stk (Ptrofs.sub (Ptrofs.repr (max_stacksize + align (size_chunk Mptr) 8)) (Ptrofs.repr (size_chunk Mptr)))) in
-      initial_state_gen p rs m (State rs0 m2).
-
-Inductive initial_state (prog: program) (rs: regset) (s: state): Prop :=
-| initial_state_intro: forall m,
-    init_mem prog = Some m ->
-    initial_state_gen prog rs m s ->
-    initial_state prog rs s.
-
-Inductive final_state: state -> int -> Prop :=
-  | final_state_intro: forall rs m r,
-      rs#PC = Vnullptr ->
-      rs#RAX = Vint r ->
-      final_state (State rs m) r.
-
-Definition semantics (p: program) (rs: regset) :=
-  Semantics_gen (step instr_size) (initial_state p rs) final_state (globalenv p) (Genv.genv_senv (globalenv p)).
-
-(** Determinacy of the [Asm] semantics. *)
-
-Lemma semantics_determinate: forall p rs, determinate (semantics p rs).
-Proof.
-Ltac Equalities :=
-  match goal with
-  | [ H1: ?a = ?b, H2: ?a = ?c |- _ ] =>
-      rewrite H1 in H2; inv H2; Equalities
-  | _ => idtac
-  end.
-  intros; constructor; simpl; intros.
-- (* determ *)
-  inv H; inv H0; Equalities.
-+ split. constructor. auto.
-+ discriminate.
-+ discriminate.
-+ assert (vargs0 = vargs) by (eapply eval_builtin_args_determ; eauto). subst vargs0.
-  exploit external_call_determ. eexact H5. eexact H11. intros [A B].
-  split. auto. intros. destruct B; auto. subst. auto.
-+ assert (args0 = args) by (eapply Asm.extcall_arguments_determ; eauto). subst args0.
-  exploit external_call_determ. eexact H3. eexact H7. intros [A B].
-  split. auto. intros. destruct B; auto. subst. auto.
-- (* trace length *)
-  red; intros; inv H; simpl.
-  lia.
-  eapply external_call_trace_length; eauto.
-  eapply external_call_trace_length; eauto.
-- (* initial states *)
-  inv H; inv H0. assert (m = m0) by congruence. subst. inv H2; inv H3.
-  assert (m1 = m3 /\ stk = stk0) by intuition congruence. destruct H0; subst.
-  assert (m2 = m4) by congruence. subst.
-  f_equal. (* congruence. *)
-- (* final no step *)
-  assert (NOTNULL: forall b ofs, Vnullptr <> Vptr b ofs).
-  { intros; unfold Vnullptr; destruct Archi.ptr64; congruence. }
-  inv H. red; intros; red; intros. inv H; rewrite H0 in *; eelim NOTNULL; eauto.
-- (* final states *)
-  inv H; inv H0. congruence.
-Qed.
-
-Theorem reloc_prog_single_events p rs:
-  single_events (semantics p rs).
-Proof.
-  red. simpl. intros s t s' STEP.
-  inv STEP; simpl. lia.
-  eapply external_call_trace_length; eauto.
-  eapply external_call_trace_length; eauto.
-Qed.
-
-Theorem reloc_prog_receptive p rs:
-  receptive (semantics p rs).
-Proof.
-  split.
-  - simpl. intros s t1 s1 t2 STEP MT.
-    inv STEP.
-    inv MT. eexists. eapply exec_step_internal; eauto.
-    edestruct external_call_receptive as (vres2 & m2 & EC2); eauto.
-    eexists. eapply exec_step_builtin; eauto.
-    edestruct external_call_receptive as (vres2 & m2 & EC2); eauto.
-    eexists. eapply exec_step_external; eauto.
-  - eapply reloc_prog_single_events; eauto.
-Qed.
-
 
 End WITH_INSTR_SIZE.
+
+
+(** Note: Builtin instructions are eliminated after AsmBuiltinInline.v . And the size of builtin instructions are unspecific *)
+(** * Evaluation of builtin arguments, *)
+
+Section EVAL_BUILTIN_ARG.
+
+Variable A: Type.
+
+Variable ge: Genv.t.
+Variable e: A -> val.
+Variable sp: val.
+Variable m:mem. 
+
+Inductive eval_builtin_arg: builtin_arg A -> val -> Prop :=
+  | eval_BA: forall x,
+      eval_builtin_arg (BA x) (e x)
+  | eval_BA_int: forall n,
+      eval_builtin_arg (BA_int n) (Vint n)
+  | eval_BA_long: forall n,
+      eval_builtin_arg (BA_long n) (Vlong n)
+  | eval_BA_float: forall n,
+      eval_builtin_arg (BA_float n) (Vfloat n)
+  | eval_BA_single: forall n,
+      eval_builtin_arg (BA_single n) (Vsingle n)
+  | eval_BA_loadstack: forall chunk ofs v,
+      Mem.loadv chunk m (Val.offset_ptr sp ofs) = Some v ->
+      eval_builtin_arg (BA_loadstack chunk ofs) v
+  | eval_BA_addrstack: forall ofs,
+      eval_builtin_arg (BA_addrstack ofs) (Val.offset_ptr sp ofs)
+  | eval_BA_loadglobal: forall chunk id ofs v,
+      Mem.loadv chunk m  (Genv.symbol_address ge id ofs) = Some v ->
+      eval_builtin_arg (BA_loadglobal chunk id ofs) v
+  | eval_BA_addrglobal: forall id ofs,
+      eval_builtin_arg (BA_addrglobal id ofs) (Genv.symbol_address ge id ofs)
+  | eval_BA_splitlong: forall hi lo vhi vlo,
+      eval_builtin_arg hi vhi -> eval_builtin_arg lo vlo ->
+      eval_builtin_arg (BA_splitlong hi lo) (Val.longofwords vhi vlo)
+  | eval_BA_addptr: forall a1 a2 v1 v2,
+      eval_builtin_arg a1 v1 ->
+      eval_builtin_arg a2 v2 ->
+      eval_builtin_arg (BA_addptr a1 a2) (if Archi.ptr64 then Val.addl v1 v2 else Val.add v1 v2).
+
+                       
+Definition eval_builtin_args (al: list (builtin_arg A)) (vl: list val) : Prop :=
+  list_forall2 eval_builtin_arg al vl.
+
+Lemma eval_builtin_arg_determ:
+  forall a v, eval_builtin_arg a v -> forall v', eval_builtin_arg a v' -> v' = v.
+Proof.
+  induction 1; intros v' EV; inv EV; try congruence.
+  f_equal; eauto.
+  destruct Archi.ptr64;f_equal;auto.
+Qed.
+
+Lemma eval_builtin_args_determ:
+  forall al vl, eval_builtin_args al vl -> forall vl', eval_builtin_args al vl' -> vl' = vl.
+Proof.
+  induction 1; intros v' EV; inv EV; f_equal; eauto using eval_builtin_arg_determ.
+Qed.
+
+ 
+End EVAL_BUILTIN_ARG.
+
+Hint Constructors eval_builtin_arg: barg.
+
+(* same lemmas as the in Events *)
+Section EVAL_BUILTIN_ARG_PRESERVED.
+
+Variables A: Type.
+Variable ge1: Genv.t.
+Variable ge2: Genv.t.
+Variable e: A -> val.
+Variable sp: val.
+Variable m: mem.
+
+Hypothesis symbols_preserved:
+  forall id, Genv.find_symbol ge2 id = Genv.find_symbol ge1 id.
+
+Lemma eval_builtin_arg_preserved:
+  forall a v, eval_builtin_arg A ge1 e sp m a v -> eval_builtin_arg A ge2 e sp m a v.
+Proof.
+   assert (EQ: forall id ofs, Genv.symbol_address ge2 id ofs = Genv.symbol_address ge1 id ofs).
+  { unfold Genv.symbol_address; simpl; intros. rewrite symbols_preserved; auto. }
+  induction 1; eauto with barg. rewrite <- EQ in H; eauto with barg. rewrite <- EQ; eauto with barg.
+Qed.
+
+Lemma eval_builtin_args_preserved:
+  forall al vl, eval_builtin_args A ge1 e sp m al vl -> eval_builtin_args A ge2 e sp m al vl.
+Proof.
+  induction 1; constructor; auto; eapply eval_builtin_arg_preserved; eauto.
+Qed.
+
+End EVAL_BUILTIN_ARG_PRESERVED.
+
+
