riscV/SymbtablegenproofArchi.v
@@ -1,9 +1,0 @@
-Require Import Coqlib Errors Maps.
-Require Import Integers Floats AST RelocProgLinking Linking.
-Require Import Values Memory Events Globalenvs Smallstep.
-Require Import Op Locations Mach Conventions Asm RealAsm.
-Require Import Symbtablegen SymbtablegenArchi.
-Require Import RelocProg RelocProgram RelocProgSemantics.
-Require Import LocalLib AsmInject.
-Import ListNotations.
-Require Import MemoryAgree.
