x86/AsmInject.v
@@ -1,9 +1,14 @@
+(* ******************* *)
+(* Author: Yuting Wang *)
+(* Date:   May 28, 2020 *)
+(* ******************* *)
+
 (** * Properties about Injections at the Asm Level *)
 
 Require Import Coqlib Errors.
 Require Import Integers Floats AST Linking.
 Require Import Values Memory Events Globalenvs Smallstep.
-Require Import Op Locations Mach Conventions Asm (* AsmFacts *).
+Require Import Op Locations Mach Conventions Asm AsmFacts.
 Require Import LocalLib.
 Import ListNotations.
 
@@ -66,7 +71,19 @@ Lemma val_inject_set:
     apply val_inject_set; auto.
     apply Val.offset_ptr_inject; auto.
   Qed.
-  
+
+  Lemma val_inject_nextinstr_nf:
+    forall j rs1 rs2 sz
+      (RINJ: forall r, Val.inject j (rs1 r) (rs2 r)) r,
+      Val.inject j (nextinstr_nf sz rs1 r) (nextinstr_nf sz rs2 r).
+  Proof.
+    unfold nextinstr_nf.
+    intros.
+    apply val_inject_nextinstr; auto.
+    intros.
+    apply val_inject_undef_regs; auto.
+  Qed.
+
 Lemma undef_regs_pres_inject : forall j rs rs' regs,
   regset_inject j rs rs' ->
   regset_inject j (Asm.undef_regs regs rs) (Asm.undef_regs regs rs').
@@ -116,6 +133,14 @@ Proof.
   unfold nextinstr. intros. apply regset_inject_expand; auto.
   apply Val.offset_ptr_inject. auto.
 Qed.  
+
+Lemma nextinstr_nf_pres_inject : forall j rs1 rs2 sz,
+    regset_inject j rs1 rs2 ->
+    regset_inject j (nextinstr_nf sz rs1) (nextinstr_nf sz rs2).
+Proof.
+  intros. apply nextinstr_pres_inject.
+  apply undef_regs_pres_inject. auto.
+Qed. 
 
 
 Lemma set_pair_pres_inject : forall j rs1 rs2 v1 v2 loc,
@@ -171,6 +196,24 @@ Ltac solve_regset_inject :=
     auto
   end.
 
+Lemma compare_floats_inject: forall j v1 v2 v1' v2' rs rs',
+    Val.inject j v1 v1' -> Val.inject j v2 v2' ->
+    regset_inject j rs rs' -> 
+    regset_inject j (compare_floats v1 v2 rs) (compare_floats v1' v2' rs').
+Proof.
+  intros. unfold compare_floats, Asm.compare_floats.
+  destruct v1, v2, v1', v2'; try solve_regset_inject. 
+Qed.
+
+Lemma compare_floats32_inject: forall j v1 v2 v1' v2' rs rs',
+    Val.inject j v1 v1' -> Val.inject j v2 v2' ->
+    regset_inject j rs rs' -> 
+    regset_inject j (compare_floats32 v1 v2 rs) (compare_floats32 v1' v2' rs').
+Proof.
+  intros. unfold compare_floats32, Asm.compare_floats32.
+  destruct v1, v2, v1', v2'; try solve_regset_inject. 
+Qed.
+
 Ltac solve_opt_lessdef := 
   match goal with
   | [ |- Val.opt_lessdef (match ?rs1 ?r with
@@ -186,6 +229,13 @@ Ltac solve_opt_lessdef :=
     generalize (H1 r); rewrite H2, H3; clear H2 H3; inversion 1; subst; solve_opt_lessdef
   | [ |- Val.opt_lessdef (Some ?v) (Some ?v) ] => constructor
   end.
+
+Lemma eval_testcond_inject: forall j c rs1 rs2,
+    regset_inject j rs1 rs2 ->
+    Val.opt_lessdef (Asm.eval_testcond c rs1) (Asm.eval_testcond c rs2).
+Proof.
+  intros. destruct c; simpl; try solve_opt_lessdef.
+Qed.
 
 (* copy from SSAsmproof *)
 (** Injection for cmpu_bool and cmplu_bool *)
@@ -297,4 +347,40 @@ Proof.
   apply Val.vofbool_inject.
 Qed.
 (* end of copy *)
+
+Lemma compare_ints_inject: forall j v1 v2 v1' v2' rs rs' m m',
+    Val.inject j v1 v1' -> Val.inject j v2 v2' ->
+    Mem.inject j m m' ->
+    regset_inject j rs rs' -> 
+    regset_inject j (compare_ints v1 v2 rs m) (compare_ints v1' v2' rs' m').
+Proof.
+  intros. unfold compare_ints, Asm.compare_ints.
+  repeat apply regset_inject_expand; auto.
+  - apply cmpu_inject; auto.
+  - apply cmpu_inject; auto.
+  - apply val_negative_inject. apply Val.sub_inject; auto.
+  - apply sub_overflow_inject; auto.
+Qed.
+
+Lemma compare_longs_inject: forall j v1 v2 v1' v2' rs rs' m m',
+    Val.inject j v1 v1' -> Val.inject j v2 v2' ->
+    Mem.inject j m m' ->
+    regset_inject j rs rs' -> 
+    regset_inject j (compare_longs v1 v2 rs m) (compare_longs v1' v2' rs' m').
+Proof.
+  intros. unfold compare_longs, Asm.compare_longs.
+  repeat apply regset_inject_expand; auto.
+  - unfold Val.cmplu.
+    exploit (cmplu_bool_lessdef j v1 v2 v1' v2' m m' Ceq); eauto. intros.
+    inversion H3; subst.
+    + simpl. auto. 
+    + simpl. apply Val.vofbool_inject.
+  - unfold Val.cmplu.
+    exploit (cmplu_bool_lessdef j v1 v2 v1' v2' m m' Clt); eauto. intros.
+    inversion H3; subst.
+    + simpl. auto. 
+    + simpl. apply Val.vofbool_inject.
+  - apply val_negativel_inject. apply Val.subl_inject; auto.
+  - apply subl_overflow_inject; auto.
+Qed.
 
